src/compiler/core/OCL_compiler_core_init.thy
@@ -267,6 +267,18 @@ subsection{* ... *}
 
 definition "activate_simp_optimization = True"
 
+definition "bootstrap_floor f_x l ocl =
+ (let (l, ocl) = f_x l ocl in
+  ( if D_generation_syntax_shallow ocl then
+      l
+    else
+      Isab_thy_generation_syntax (Generation_syntax_shallow (D_design_analysis ocl))
+      # Isab_thy_ml_extended (Ml_extended (Sexpr_ocl (ocl \<lparr> D_disable_thy_output := True
+                                                          , D_file_out_path_dep := None
+                                                          , D_output_position := (0, 0) \<rparr>) ))
+      # l
+  , ocl \<lparr> D_generation_syntax_shallow := True \<rparr> ))"
+
 subsection{* Infra *}
 
 fun print_infra_type_synonym_class_rec_aux0 where
@@ -353,6 +365,8 @@ definition "raise_ml l_out s = Ml (Sexpr_apply \<open>Ty'.check\<close>
                      (Sexpr_string s))
         l_out
     , Sexpr_string s ])"
+
+definition "print_examp_def_st_inst_var_name ocli name = flatten [case Inst_name ocli of Some n \<Rightarrow> n, name]"
 
 subsection{* context *}
 
