src/compiler/core/OCL_compiler_floor2_examp.thy
@@ -1,0 +1,311 @@
+(*****************************************************************************
+ * Featherweight-OCL --- A Formal Semantics for UML-OCL Version OCL 2.5
+ *                       for the OMG Standard.
+ *                       http://www.brucker.ch/projects/hol-testgen/
+ *
+ * OCL_compiler_floor2_examp.thy ---
+ * This file is part of HOL-TestGen.
+ *
+ * Copyright (c) 2013-2015 Université Paris-Sud, France
+ *               2013-2015 IRT SystemX, France
+ *
+ * All rights reserved.
+ *
+ * Redistribution and use in source and binary forms, with or without
+ * modification, are permitted provided that the following conditions are
+ * met:
+ *
+ *     * Redistributions of source code must retain the above copyright
+ *       notice, this list of conditions and the following disclaimer.
+ *
+ *     * Redistributions in binary form must reproduce the above
+ *       copyright notice, this list of conditions and the following
+ *       disclaimer in the documentation and/or other materials provided
+ *       with the distribution.
+ *
+ *     * Neither the name of the copyright holders nor the names of its
+ *       contributors may be used to endorse or promote products derived
+ *       from this software without specific prior written permission.
+ *
+ * THIS SOFTWARE IS PROVIDED BY THE COPYRIGHT HOLDERS AND CONTRIBUTORS
+ * "AS IS" AND ANY EXPRESS OR IMPLIED WARRANTIES, INCLUDING, BUT NOT
+ * LIMITED TO, THE IMPLIED WARRANTIES OF MERCHANTABILITY AND FITNESS FOR
+ * A PARTICULAR PURPOSE ARE DISCLAIMED. IN NO EVENT SHALL THE COPYRIGHT
+ * OWNER OR CONTRIBUTORS BE LIABLE FOR ANY DIRECT, INDIRECT, INCIDENTAL,
+ * SPECIAL, EXEMPLARY, OR CONSEQUENTIAL DAMAGES (INCLUDING, BUT NOT
+ * LIMITED TO, PROCUREMENT OF SUBSTITUTE GOODS OR SERVICES; LOSS OF USE,
+ * DATA, OR PROFITS; OR BUSINESS INTERRUPTION) HOWEVER CAUSED AND ON ANY
+ * THEORY OF LIABILITY, WHETHER IN CONTRACT, STRICT LIABILITY, OR TORT
+ * (INCLUDING NEGLIGENCE OR OTHERWISE) ARISING IN ANY WAY OUT OF THE USE
+ * OF THIS SOFTWARE, EVEN IF ADVISED OF THE POSSIBILITY OF SUCH DAMAGE.
+ ******************************************************************************)
+(* $Id:$ *)
+
+header{* Part ... *}
+
+theory  OCL_compiler_floor2_examp
+imports OCL_compiler_floor1_examp
+begin
+
+section{* Translation of AST *}
+
+subsection{* example *}
+
+definition "print_examp_def_st_defassoc_typecheck_gen l ocl =
+ ([ raise_ml
+      (case
+         List.fold
+           (\<lambda> OclDefCoreBinding name \<Rightarrow>
+            \<lambda>(l, rbt).
+             ( ( (if List.assoc name (D_instance_rbt ocl) = None then
+                    Cons (Error, name)
+                  else
+                    id)
+               o (if lookup rbt name = None then
+                    id
+                  else
+                    Cons (Warning, name))) l
+             , insert name () rbt))
+           l
+           ([], RBT.empty)
+       of
+         ([], _) \<Rightarrow> []
+       | (l, _) \<Rightarrow> rev_map (\<lambda> (Error, n) \<Rightarrow> (Error, \<open>Extra variables on rhs: \<close> @@ n)
+                            | (Warning, n) \<Rightarrow> (Warning, \<open>Duplicate variables on rhs: \<close> @@ n)) l)
+      \<open> error(s)\<close> ])"
+
+definition "print_examp_def_st_defassoc_typecheck = (\<lambda> OclDefSt _ l \<Rightarrow> \<lambda> ocl.
+  (\<lambda>l_res. (List_map Thy_ml l_res, ocl \<lparr> D_import_compiler := True \<rparr>))
+  (print_examp_def_st_defassoc_typecheck_gen
+    l
+    ocl))"
+
+definition "print_examp_def_st_mapsto_gen f ocl cpt_start =
+  List_map
+    (\<lambda>(cpt, ocore).
+        let a = \<lambda>f x. Expr_apply f [x]
+          ; b = \<lambda>s. Expr_basic [s]
+          ; (ocli, exp) = case ocore of
+            OclDefCoreBinding (name, ocli) \<Rightarrow> (ocli, Some (let\<^sub>O\<^sub>C\<^sub>a\<^sub>m\<^sub>l name = print_examp_instance_name (\<lambda>s. s @@ isub_of_str (Inst_ty ocli)) name in
+                                                           if D_design_analysis ocl = Gen_only_design then
+                                                             a name cpt_start
+                                                           else
+                                                             b name)) in
+        f (cpt, ocore) ocli exp)"
+
+definition "print_examp_def_st_mapsto ocl name l =
+  list_bind id id (print_examp_def_st_mapsto_gen
+    (\<lambda>(cpt, _) ocli. map_option (\<lambda>exp.
+      Expr_binop (Expr_oid var_oid_uniq (oidGetInh cpt)) \<open>\<mapsto>\<close> (Expr_apply (datatype_in @@ isub_of_str (Inst_ty ocli)) [exp])))
+    ocl
+    name
+    l)"
+
+definition "print_examp_def_st_defassoc_name name = Expr_basic [flatten [var_inst_assoc, name]]"
+definition "print_examp_def_st_defassoc = (\<lambda> OclDefSt name l \<Rightarrow> \<lambda>ocl.
+ let l_ocli = List.map_filter (\<lambda> OclDefCoreBinding name \<Rightarrow>
+                                   List.assoc name (D_instance_rbt ocl)) l in
+ (\<lambda>l. (print_examp_instance_oid l_ocli ocl @@@@ List_map Thy_definition_hol l, ocl))
+  (print_examp_instance_defassoc_gen
+    (print_examp_def_st_defassoc_name name)
+    l_ocli
+    (ocl \<lparr> D_oid_start := oidReinitInh (D_oid_start ocl) \<rparr>)))"
+
+definition "print_examp_def_st2 = (\<lambda> OclDefSt name l \<Rightarrow> \<lambda>ocl.
+ (\<lambda>(l, l_st). (List_map Thy_definition_hol l, ocl \<lparr> D_state_rbt := (String_to_String\<^sub>b\<^sub>a\<^sub>s\<^sub>e name, l_st) # D_state_rbt ocl \<rparr>))
+  (let b = \<lambda>s. Expr_basic [s]
+     ; l = List_map (\<lambda> OclDefCoreBinding name \<Rightarrow> map_option (Pair name) (List.assoc name (D_instance_rbt ocl))) l
+     ; (rbt, (map_self, map_username)) =
+         (init_map_class 
+           (ocl \<lparr> D_oid_start := oidReinitInh (D_oid_start ocl) \<rparr>)
+           (List_map (\<lambda> Some (_, ocli, _) \<Rightarrow> ocli | None \<Rightarrow> ocl_instance_single_empty) l)
+          :: (_ \<Rightarrow> _ \<times> (_ \<Rightarrow> ((_ \<Rightarrow> nat \<Rightarrow> _ \<Rightarrow> _) \<Rightarrow> _
+                        \<Rightarrow> (ocl_ty_class option \<times> (ocl_ty \<times> ocl_data_shallow) option) list) option)) \<times> _ \<times> _)
+     ; (l_st, l_assoc) = fold_list (\<lambda> o_n l_assoc.
+           case o_n of
+              Some (name, ocli, cpt) \<Rightarrow> ([(cpt, OclDefCoreBinding (name, ocli))], (ocli, cpt) # l_assoc)
+            | None \<Rightarrow> ([], l_assoc)) l []
+     ; l_st = List_unique oidGetInh (List_flatten l_st)
+     ; expr_app = print_examp_def_st_mapsto ocl (print_examp_def_st_defassoc_name name) l_st in
+
+   ( [ let s_empty = \<open>Map.empty\<close> in
+       Definition (Expr_rewrite (b name) \<open>=\<close> (Expr_apply \<open>state.make\<close>
+        ( Expr_apply s_empty (case expr_app of None \<Rightarrow> [] | Some l \<Rightarrow> l)
+        # [ if D_design_analysis ocl = Gen_only_design then
+              b s_empty
+            else
+              print_examp_def_st_assoc rbt map_self map_username l_assoc ]))) ]
+   , l_st)))"
+
+definition "print_examp_def_st_inst_var = (\<lambda> OclDefSt name l \<Rightarrow> \<lambda> ocl.
+ let ocl_old = ocl \<lparr> D_oid_start := oidReinitInh (D_oid_start ocl) \<rparr>
+   ; l_ocli = List_map (\<lambda> OclDefCoreBinding name \<Rightarrow>
+                            map_option fst (List.assoc name (D_instance_rbt ocl_old))) l in
+  (\<lambda>l_res. ((List_map Thy_definition_hol o List_flatten) l_res, ocl))
+    (let ocl = ocl_old in
+     case D_design_analysis ocl of Gen_only_analysis \<Rightarrow> [] | Gen_default \<Rightarrow> [] | Gen_only_design \<Rightarrow>
+     fst (fold_list
+      (\<lambda> (f1, f2) _.
+        let (l, accu) =
+        fold_list (\<lambda> ocli cpt.
+          ( case ocli of None \<Rightarrow> [] | Some ocli \<Rightarrow>
+              let\<^sub>O\<^sub>C\<^sub>a\<^sub>m\<^sub>l var_oid = Expr_oid var_oid_uniq (oidGetInh cpt)
+                ; isub_name = \<lambda>s. s @@ isub_of_str (Inst_ty ocli) in
+              [Definition (Expr_rewrite (f1 var_oid isub_name ocli) \<open>=\<close> (f2 ocli isub_name cpt))]
+          , oidSucInh cpt)) l_ocli (D_oid_start ocl) in
+          (List_flatten l, accu))
+      (let a = \<lambda>f x. Expr_apply f [x]
+         ; b = \<lambda>s. Expr_basic [s] in
+       [ (\<lambda> _ _ ocli. Expr_annot (b (flatten [inst_name ocli, name])) (Inst_ty ocli),
+          \<lambda> ocli isub_name _. Expr_lambda wildcard (Expr_some (Expr_some (a (print_examp_instance_name isub_name (inst_name ocli))
+                                                                            (print_examp_def_st_defassoc_name name))))) ])
+      (D_oid_start ocl))))"
+
+definition "print_examp_def_st_dom_name name = flatten [\<open>dom_\<close>, name]"
+definition "print_examp_def_st_dom = (\<lambda> _ ocl.
+ (\<lambda> l. (List_map Thy_lemma_by l, ocl))
+  (let (name, l_st) = map_prod String\<^sub>b\<^sub>a\<^sub>s\<^sub>e_to_String id (hd (D_state_rbt ocl))
+     ; a = \<lambda>f x. Expr_apply f [x]
+     ; b = \<lambda>s. Expr_basic [s]
+     ; d = hol_definition in
+   [ Lemma_by
+       (print_examp_def_st_dom_name name)
+       [Expr_rewrite (a \<open>dom\<close> (a \<open>heap\<close> (b name))) \<open>=\<close> (Expr_set (List_map (\<lambda>(cpt, _). Expr_oid var_oid_uniq (oidGetInh cpt)) l_st))]
+       []
+       (Tacl_by [Tac_auto_simp_add [d name]])]))"
+
+definition "print_examp_def_st_dom_lemmas = (\<lambda> _ ocl.
+ (\<lambda> l. (List_map Thy_lemmas_simp l, ocl))
+  (let (name, _) = hd (D_state_rbt ocl) in
+   [ Lemmas_simp \<open>\<close>
+       [Thm_str (print_examp_def_st_dom_name (String\<^sub>b\<^sub>a\<^sub>s\<^sub>e_to_String name))] ]))"
+
+definition "print_examp_def_st_perm_name name = flatten [\<open>perm_\<close>, name]"
+definition "print_examp_def_st_perm = (\<lambda> _ ocl.
+ (\<lambda> l. (List_map Thy_lemma_by l, ocl))
+  (let (name, l_st) = map_prod String\<^sub>b\<^sub>a\<^sub>s\<^sub>e_to_String id (hd (D_state_rbt ocl))
+     ; expr_app = let ocl = ocl \<lparr> D_oid_start := oidReinitInh (D_oid_start ocl) \<rparr> in
+                  print_examp_def_st_mapsto
+                    ocl
+                    (print_examp_def_st_defassoc_name name)
+                    (rev l_st)
+     ; a = \<lambda>\<^sub>S\<^sub>c\<^sub>a\<^sub>l\<^sub>af x. Expr_apply f [x]
+     ; b = \<lambda>s. Expr_basic [s]
+     ; d = hol_definition
+     ; (l_app, l_last) =
+         case l_st of [] \<Rightarrow> ([], Tacl_by [Tac_simp_add [d name]])
+         | [_] \<Rightarrow> ([], Tacl_by [Tac_simp_add [d name]])
+         | _ \<Rightarrow>
+           ( [ Tac_simp_add (List_map d (name # List_map (\<lambda>(cpt, _). var_oid_uniq @@ natural_of_str (case oidGetInh cpt of Oid i \<Rightarrow> i)) l_st))]
+             # List_flatten (List_map (\<lambda>i_max. List_map (\<lambda>i. [Tac_subst_l (List_map nat_of_str [i_max - i]) (Thm_str \<open>fun_upd_twist\<close>), Tac_simp]) (List.upt 0 i_max)) (List.upt 1 (List.length l_st)))
+           , Tacl_by [Tac_simp]) in
+   case expr_app of None \<Rightarrow> [] | Some expr_app \<Rightarrow>
+   [ Lemma_by
+       (print_examp_def_st_perm_name name)
+       [Expr_rewrite (b name) \<open>=\<close> (Expr_apply \<open>state.make\<close>
+          (let s_empty = \<open>Map.empty\<close> in
+           Expr_apply s_empty expr_app # [Expr_apply var_assocs [b name]]))]
+       l_app
+       l_last ]))"
+
+definition "extract_state ocl name_st l_st =
+ (let b = \<lambda>s. Expr_basic [s]
+    ; ocl = ocl \<lparr> D_oid_start := oidReinitInh (D_oid_start ocl) \<rparr> in
+  print_examp_def_st_mapsto_gen
+                    (\<lambda>(_, ocore) ocli exp.
+                      ( ocore
+                      , ocli
+                      , case ocore of
+                          OclDefCoreBinding (name, ocli) \<Rightarrow>
+                            b (if D_design_analysis ocl = Gen_only_design then
+                                 print_examp_def_st_inst_var_name ocli name_st
+                               else
+                                 name)))
+                    ocl
+                    (print_examp_def_st_defassoc_name name_st)
+                    l_st)"
+
+definition "print_examp_def_st_allinst = (\<lambda> _ ocl.
+ (\<lambda> l. (List_map Thy_lemma_by l, ocl))
+  (let (name_st, l_st) = map_prod String\<^sub>b\<^sub>a\<^sub>s\<^sub>e_to_String id (hd (D_state_rbt ocl))
+     ; b = \<lambda>s. Expr_basic [s]
+     ; expr_app = extract_state ocl name_st l_st
+     ; a = \<lambda>f x. Expr_apply f [x]
+     ; d = hol_definition
+     ; l_st_oid = List_map (\<lambda>(cpt, _). var_oid_uniq @@ natural_of_str (case oidGetInh cpt of Oid i \<Rightarrow> i)) l_st in
+   map_class_gen_h'_inh (\<lambda> isub_name name compare.
+     let expr_app = List_map (\<lambda>(ocore, ocli, exp).
+              ( ocore
+              , let exp_annot = [(Expr_postunary (case ocore of OclDefCoreBinding _ \<Rightarrow> exp) (b (dot_astype name)), True, ocore)] in
+                case compare (Inst_ty ocli) of
+                  EQ \<Rightarrow> [(exp, False, ocore)]
+                | LT \<Rightarrow> exp_annot
+                | GT \<Rightarrow> (case Inst_attr ocli of OclAttrCast name2 _ _ \<Rightarrow>
+                           if String_equal name name2 then exp_annot
+                           else [] | _ \<Rightarrow> [])
+                | UN' \<Rightarrow> [])) expr_app
+       ; (l_spec, l_body) = List_split (List_flatten (List_map snd expr_app)) in
+     gen_pre_post
+       (\<lambda>s. flatten [ name_st, \<open>_\<close>, s, \<open>_exec_\<close>, name ])
+       (\<lambda>f_expr f_mk _. Expr_binop
+            (f_mk (b name_st))
+            \<open>\<Turnstile>\<close>
+            (Expr_binop (f_expr [b name]) \<open>\<doteq>\<close> (Expr_oclset l_spec)))
+       (\<lambda>lem_tit lem_spec var_pre_post var_mk _. Lemma_by_assum
+         lem_tit
+         [(\<open>\<close>, True, Expr_And \<open>a\<close> (\<lambda>var_a. Expr_rewrite (a var_pre_post (a var_mk (b var_a))) \<open>=\<close> (b var_a)))]
+         lem_spec
+         (List_map App
+           (List_flatten
+            [ [[Tac_subst (Thm_str (print_examp_def_st_perm_name name_st))]]
+            , [[Tac_simp_only
+                 (List_map
+                   (Thm_str o d)
+                   (List_flatten
+                      [ [\<open>state.make\<close>]
+                      , l_st_oid
+                      , List_flatten (List_map (\<lambda>(_, ocore).
+                          case ocore of
+                            OclDefCoreBinding (n, ocli) \<Rightarrow>
+                              [if D_design_analysis ocl = Gen_only_design then
+                                 print_examp_def_st_inst_var_name ocli name_st
+                               else
+                                 n]) l_body)
+                      , List_flatten (List_map (\<lambda>(cast, ocore).
+                          if cast then
+                            case
+                              case ocore of OclDefCoreBinding (_, ocli) \<Rightarrow> Some ocli
+                            of Some ocli \<Rightarrow> [print_examp_instance_name (\<lambda>s. s @@ isub_of_str (Inst_ty ocli)) (inst_name ocli)]
+                             | None \<Rightarrow> []
+                          else []) l_body) ]))]]
+            , fst (fold_list (\<lambda> expr l_spec.
+                let mk_StrictRefEq_including = \<lambda>l.
+                      Tac_rule (Thm_str \<open>const_StrictRefEq\<^sub>S\<^sub>e\<^sub>t_including\<close>)
+                      # Tac_simp # Tac_simp # Tac_simp # l
+                  ; (state_update_vs_allInstances_generic, l_spec, l_print_examp, l_OclIncluding_cong) =
+                  case expr of (ocore, []) \<Rightarrow>
+                    ( \<open>state_update_vs_allInstances_generic_ntc\<close>
+                    , l_spec
+                    , case ocore of OclDefCoreBinding (_, ocli) \<Rightarrow> [print_examp_instance_name (\<lambda>s. s @@ isub_of_str (Inst_ty ocli)) (inst_name ocli)]
+                    , if l_spec = [] then
+                        [Tac_rule (Thm_str \<open>const_StrictRefEq\<^sub>S\<^sub>e\<^sub>t_empty\<close>), Tac_simp]
+                      else
+                        mk_StrictRefEq_including [])
+                  | _ \<Rightarrow>
+                    ( \<open>state_update_vs_allInstances_generic_tc\<close>
+                    , tl l_spec
+                    , []
+                    , mk_StrictRefEq_including [ Tac_rule (Thm_str \<open>OclIncluding_cong\<close>), Tac_simp, Tac_simp ]) in
+                ( Tac_subst (Thm_str state_update_vs_allInstances_generic)
+                  # Tac_simp # Tac_simp
+                  # Tac_simp_add (List_map d ((flatten [isub_name const_oclastype, \<open>_\<AA>\<close>]) # l_print_examp))
+                  # Tac_simp
+                  # l_OclIncluding_cong
+                , l_spec) ) expr_app l_spec)
+            , [[Tac_rule (Thm_str \<open>state_update_vs_allInstances_generic_empty\<close>)]] ]))
+         (Tacl_by [ if l_spec = [] then Tac_simp
+                    else Tac_simp_all_add [d (flatten [isub_name const_oclastype, \<open>_\<AA>\<close>])]]) )
+       [Tac_simp])
+     (case D_class_spec ocl of Some class_spec \<Rightarrow> class_spec)))"
+
+end
