src/compiler/meta/OCL_compiler_meta_META.thy
@@ -76,7 +76,7 @@ datatype ocl_deep_embed_ast =
                               (* invented *)
                             | OclAstInstance ocl_instance
                             | OclAstDefBaseL ocl_def_base_l
-                            | OclAstDefState ocl_def_state
+                            | OclAstDefState floor ocl_def_state
                             | OclAstDefPrePost ocl_def_pre_post
                             | OclAstFlushAll ocl_flush_all
 
